\section*{Lemma 2:}

With probability larger than $1-\frac{2}{n}$ it holds that

\begin{center}
$|\langle E^2, B^*-B \rangle| \le (7.(C^2+1).[\sum_{j\neq k}|B_{G_jG_k}|_1].\frac{d}{\sqrt{m}})$
\end{center}

With $d=\mbox{max}(n.\mbox{max}_{i,j} C_{ij}, \mbox{ln}n)$

\section*{Proof:}

if we do the same of (58) we have :
\begin{align*}
|\langle E^2, B^*-B \rangle| \le 2.[\sum_{j\neq k}|B_{G_jG_k}|_1](3.|B^*E^2|_{\infty} + \frac{||E^2||_{op}}{2m})
\end{align*}

\begin{align*}
||E^2||_{op} &= ||E||_{op}^2 \le 2.(||\mathcal{E}||_{op}^2 + |D|_{\infty}^2)
\end{align*}

for all $a$ in $G_k$:
\begin{align*}
|[B^*E^2]_{a:}|_{\infty} &= \frac{1}{|G_k|}|[E^2.1_{G_k}]|_{\infty} \\ &\le \frac{1}{|G_k|}||[E^2.1_{G_k}]||_2 \le \frac{1}{|G_k|}||E^2||_{op}||1_{G_k}||_2 \\ & \le \frac{1}{\sqrt{m}}||E^2||_{op}
\end{align*}

And :

\begin{align*}
|B^*E^2|_{\infty} &= \mbox{max}_{a}|[B^*E^2]_{a:}|_{\infty} \\ & \le \frac{1}{\sqrt{m}}||E^2||_{op}
\end{align*}

Hence :
\begin{align*}
|\langle E^2, B^*-B \rangle| \le 7.[\sum_{j\neq k}|B_{G_jG_k}|_1].\frac{||\mathcal{E}||_{op}^2 + |D|_{\infty}^2}{\sqrt{m}}
\end{align*}

We use the Theorem 5.1 
With probability $1-\frac{2}{n}$
\begin{align*}
||\mathcal{E}||_{op} \le C\sqrt{d}
\end{align*}

And : $|D|_{\infty}^2 \le d$

So : 
\begin{align*}
|\langle E^2, B^*-B \rangle| \le 7.(C^2+1).[\sum_{j\neq k}|B_{G_jG_k}|_1].\frac{d}{\sqrt{m}}
\end{align*}